TM/Combinators/SequentialComposition.v
@@ -33,6 +33,34 @@ Section Composition.
     intros H1 H2. eapply Match_Terminates'; eauto.
   Qed.
 
+  Section Seq_Terminates.
+
+    Variable (T1 : (tapes sig n) -> nat -> Type).
+    Variable (T2 : (tapes sig n) -> nat -> Type).
+
+    Hypothesis (Term1 : projT1 pM1 ⇓ T1).
+    Hypothesis (Term2 : projT1 pM2 ⇓ T2).
+
+    Record Seq_Terminates_Rel (t : tapes sig n) (k'' : nat) : Type :=
+      {
+        term_k : nat;
+        term_k' : nat;
+        term_In : term_k + term_k' < k'';
+        term_m1 : T1 t term_k;
+        term_m2 : T2 (ctapes (proj1_sig (Term1 term_m1))) term_k';
+      }.
+
+    Lemma Seq_Terminates :
+      projT1 Seq ⇓ Seq_Terminates_Rel.
+    Proof.
+      unfold Seq, MATCH. cbn.
+      eapply TerminatesIn_monotone.
+      - apply Match_Terminates. instantiate (1 := fun _ => T2). auto. Unshelve. apply T1. apply Term1.
+      - intros t k''. intros [k k' H1 H2 H3]. econstructor; eauto.
+    Qed.
+
+  End Seq_Terminates.
+
   Lemma Seq_RealiseIn (R1 : Rel _ _) (R2 : Rel _ (F2 * _)) k1 k2:
     pM1 ⊨c(k1) R1 ->
     pM2 ⊨c(k2) R2 ->
